# Aula 28/03

### Cones

**Cone:** $A$ é cone $\Leftrightarrow \forall(a, \lambda) \in A \times \mathbb{R}_+ \Rightarrow \lambda a \in A$

**Cone gerado:** $C(A) := \{\lambda a: a \in A , \lambda \in \mathbb{R}_+\}$

**Propriedade 9:** $A$ convexo \Rightarrow $C(A)$ é convexo
\[
    \forall(c^1, c^2, \lambda) \in C(A) \times C(A) \times [0, 1] \\
    c_\lambda := \lambda c^1 + (1-\lambda)c^2 \\
    \exists (a^1, a^2, \beta_1, \beta_2) \in A \times A \times \mathbb{R}_+ \times \mathbb{R}_+ \\
    c^i = \beta_i a^i \quad i = 1, 2 \\
\]

>Queremos
>
\[
    \beta \bar{a} = c_\lambda = \lambda c^1 + (1-\lambda)c^2 \\
    \bar{a} = \alpha a^1 + (1-\alpha)a^2 \\
    \beta \alpha a^1 + \beta(1-\alpha)a^2 = \lambda c^1 + (1-\lambda c^2) = \beta_1 \lambda a^1 + \beta_2(1- \lambda)a^2\\
    \left.\begin{array}\beta \alpha = \beta_1 \lambda \\
    \beta(1-\alpha) = \beta_2(1 - \lambda)\end{array}\right\} \beta = \beta_2(1-\lambda) + \beta_1 \lambda = \lambda\beta_1 + (1-\lambda)\beta_2 \\
    \Rightarrow \alpha = \frac{\beta_1 \lambda}{\lambda\beta_1 + (1-\lambda)\beta_2} \\
\]

Sejam $\alpha = \frac{\beta_1 \lambda}{\lambda\beta_1 + (1-\lambda)\beta_2}\in [0, 1]$, $\beta = \lambda\beta_1 + (1-\lambda)\beta_2 \geq 0$ e $\bar{a} := \alpha a^1 + (1-\alpha)a^2 \in A \text{ (convexo)}$

Além disso,
\[
    \beta\bar{a}= \beta\alpha a^1 + \beta (1-\alpha)a^2 = \\
     (\lambda\beta_1 + (1-\lambda)\beta_2)\left(\frac{\beta_1 \lambda}{\lambda\beta_1 + (1-\lambda)\beta_2}\right)a^1 + (\lambda\beta_1 + (1-\lambda)\beta_2 ) \left(1 - \frac{\beta_1 \lambda}{\lambda\beta_1 + (1-\lambda)\beta_2}\right)a^2 \\
     = \lambda\beta_1 a^1 + (1- \lambda)\beta_2 a^2 = c_\lambda
\]
